chore: add definitions needed to be able to define arm state for example
I next need to write down the correctness statement, but I'm really
not sure where the effect of 'ret' is recorded. Does 'ret' store into
some blessed register as per calling convention?

Arm/State.lean
@@ -27,6 +27,12 @@ def write_store {α β : Type} [DecidableEq α]
   (a : α) (b : β) (store : Store α β) : Store α β :=
   fun x => if x = a then b else (store x)
 
+/-- A store that stores a single value `b`. This is a constant function -/
+def Store.const (b : β) : Store α β := fun _ => b
+
+@[simp]
+theorem Store.read_const [DecidableEq α] (b : β) (a : α) : read_store a (Store.const b) = b := rfl
+
 -- Let's have these theorems added to simp, but local only to this file.
 @[local simp]
 theorem store_read_over_write_same [DecidableEq α] (a : α) (b : β) (store : Store α β) :
@@ -115,6 +121,15 @@ structure PState where
   v : BitVec 1
 deriving DecidableEq, Repr
 
+def PState.default : PState where 
+  n := 0#1
+  z := 0#1
+  c := 0#1
+  v := 0#1
+
+instance : Inhabited PState where 
+  default := PState.default
+
 @[ext]
 structure ArmState where
   -- General-purpose registers: register 31 is the stack pointer.
@@ -138,6 +153,18 @@ structure ArmState where
   -- execution based off an erroneous state is invalid.
   error      : StateError
 deriving Repr
+
+def ArmState.default : ArmState where 
+  gpr := .const 0
+  sfp := .const 0
+  pc := 0#64
+  pstate := .default
+  mem := .const 0
+  error := .None
+  program := []
+
+instance : Inhabited ArmState where 
+  default := .default
 
 ---- Basic State Accessors and Updaters (except memory) ----
 
